examples/echo(wip): Start working on conditionals

src/Rupicola/Examples/Echo/Echo.v
@@ -19,12 +19,18 @@ Section Echo.
   Definition putw_trace (w: word) : trace_entry :=
     (map.empty (map := mem), "putw", [w], (map.empty, [])).
 
+  Definition trace_entry_of_event (evt: IO.Event word) :=
+    match evt with
+    | IO.R t => getw_trace t
+    | IO.W t => putw_trace t
+    end.
+
   Instance spec_of_getw : spec_of "getw" :=
     fnspec! "getw" ~> r,
     { requires tr mem := True;
       ensures tr' mem' :=
         mem' = mem /\
-        tr' = getw_trace r :: tr }.
+        tr' = trace_entry_of_event (IO.R r) :: tr }.
 
   Instance spec_of_putw : spec_of "putw" :=
     fnspec! "putw" w ~> r,
@@ -32,20 +38,15 @@ Section Echo.
       ensures tr' mem' :=
         mem' = mem /\
         r = word.of_Z 0 /\
-        tr' = putw_trace w :: tr }.
-
-  Definition trace_entry_of_event (evt: IO.Event word) :=
-    match evt with
-    | IO.R t => getw_trace t
-    | IO.W t => putw_trace t
-    end.
+        tr' = trace_entry_of_event (IO.W w) :: tr }.
 
   Notation IO := (IO.M word).
+  Notation iospec := (iospec trace_entry_of_event).
   Notation iospec_k := (iospec_k trace_entry_of_event).
 
   Lemma compile_getw : forall {tr mem locals functions},
     let io: IO _ := Free.Call IO.Read in
-    forall {A} {pred: A -> predicate}
+    forall {A} {pred: A -> pure_predicate}
       {k: word -> IO A} {k_impl}
       var,
 
@@ -69,6 +70,7 @@ Section Echo.
         k_impl
       <{ iospec_k tr pred (mbindn [var] io k) }>.
   Proof.
+    set (IO.Read).
     repeat straightline.
     straightline_call; eauto; [].
     repeat straightline; subst_lets_in_goal.
@@ -80,7 +82,7 @@ Section Echo.
 
   Lemma compile_putw : forall {tr mem locals functions} (w: word),
     let io: IO unit := Free.Call (IO.Write w) in
-    forall {A} {pred: A -> predicate}
+    forall {A} {pred: A -> pure_predicate}
       {k: unit -> IO A} {k_impl}
       w_expr var,
 
@@ -117,31 +119,75 @@ Section Echo.
     - intros; eassumption.
   Qed.
 
-  Definition io_sum : IO unit :=
-    let/! w1 := IO.Read in
-    let/! w2 := IO.Read in
-    let/n sum := word.add w1 w2 in
-    let/! _ := IO.Write sum in
-    mret tt.
-
-  Instance spec_of_hello_word : spec_of "io_sum" :=
-    fnspec! "io_sum" / (R: mem -> Prop),
-    { requires tr mem :=
-        R mem;
-      ensures tr' mem' rets :=
-        iospec trace_entry_of_event tr io_sum (fun val tr'' => tr' = tr'' /\ R mem') }.
-
   Hint Extern 1 => simple eapply compile_putw; shelve : compiler.
   Hint Extern 1 => simple eapply compile_getw; shelve : compiler.
 
+  Definition io_echo : IO unit :=
+    let/! w := call! IO.Read in
+    let/! _ := call! IO.Write w in
+    mret tt.
+
+  Instance spec_of_io_echo : spec_of "io_echo" :=
+    fnspec! "io_echo" / (R: mem -> Prop),
+    { requires tr mem := R mem;
+      ensures tr' mem' rets := iospec tr tr' io_echo (fun _ => R mem') }.
+
+  Derive io_echo_body SuchThat
+   (defn! "io_echo"() { io_echo_body },
+    implements io_echo using ["getw"; "putw"])
+   As io_echo_target_correct.
+  Proof. compile. Qed.
+
+  Definition io_sum : IO unit :=
+    let/! w1 := call! IO.Read in
+    let/! w2 := call! IO.Read in
+    let/n sum := word.add w1 w2 in
+    let/! _ := call! IO.Write sum in
+    mret tt.
+
+  Instance spec_of_io_sum : spec_of "io_sum" :=
+    fnspec! "io_sum" / (R: mem -> Prop),
+    { requires tr mem := R mem;
+      ensures tr' mem' rets := iospec tr tr' io_sum (fun _ => R mem') }.
+
   Derive io_sum_body SuchThat
-         (defn! "io_sum"()
-              { io_sum_body },
+         (defn! "io_sum"() { io_sum_body },
           implements io_sum using ["getw"; "putw"])
   As io_sum_target_correct.
+  Proof. compile. Qed.
+
+  Open Scope Z_scope.
+
+  Definition io_check expected : IO word :=
+    let/! read := call! IO.Read in
+    let/! err := if word.eqb (word := word) read expected
+                then let/! _ := call! IO.Write (word.of_Z 0) in
+                     mret (word.of_Z 0)
+                else let/! _ := call! IO.Write (word.of_Z 42) in
+                     mret (word.of_Z 42) in
+    mret err.
+
+  Instance spec_of_io_check : spec_of "io_check" :=
+    fnspec! "io_check" expected / (R: mem -> Prop),
+    { requires tr mem := R mem;
+      ensures tr' mem' rets := iospec tr tr' (io_check expected) (fun val => rets = [val] /\ R mem') }.
+
+  Derive io_check_body SuchThat
+         (defn! "io_check"("expected") { io_check_body },
+          implements io_check using ["getw"; "putw"])
+  As io_check_target_correct.
   Proof.
-    compile.
+    compile_setup.
+    compile_step.
+    compile_step.
+    compile_step.
+    compile_step.
+    eapply compile_if.
+    repeat compile_step.
+    (* FIXME rewrite bind_bind *)
   Qed.
+
+
 End Echo.
 
 Require Import bedrock2.NotationsCustomEntry.
